cardano-mpfs-offchain/test/Cardano/MPFS/StateSpec.hs
@@ -168,9 +168,9 @@ checkpointsSpec newCheckpoints = do
             forAll genBlockId $ \b ->
                 monadicIO $ do
                     cp <- run newCheckpoints
-                    run $ putCheckpoint cp s b
+                    run $ putCheckpoint cp s b []
                     r <- run $ getCheckpoint cp
-                    assert (r == Just (s, b))
+                    assert (r == Just (s, b, []))
 
     prop "put overwrites previous"
         $ forAll genSlotNo
@@ -180,7 +180,18 @@ checkpointsSpec newCheckpoints = do
                     forAll genBlockId $ \b2 ->
                         monadicIO $ do
                             cp <- run newCheckpoints
-                            run $ putCheckpoint cp s1 b1
-                            run $ putCheckpoint cp s2 b2
+                            run
+                                $ putCheckpoint
+                                    cp
+                                    s1
+                                    b1
+                                    []
+                            run
+                                $ putCheckpoint
+                                    cp
+                                    s2
+                                    b2
+                                    []
                             r <- run $ getCheckpoint cp
-                            assert (r == Just (s2, b2))
+                            assert
+                                (r == Just (s2, b2, []))
